starting the integration of abrupt termination.. Not finished since lattice stuff is missing!

C-verifier/src/Midend-IVL/Isabelle-UTP-Extended/impl/utp_prog_abrupt_more.thy
@@ -14,39 +14,37 @@
  * See CONTRIBUTORS, LICENSE and CITATION files for details.
  ******************************************************************************)
 
-section {* Imperative Programs *}
+section \<open>Imperative Programs\<close>
   
 theory utp_prog_abrupt_more
   imports 
     "../HoareLogic/TotalCorrectness/utp_hoare_ndes_prog"
 begin
 
-section {*Abrupt*}
-subsection {*Sequential C-program alphabet*}
+section \<open>Abrupt\<close>
+subsection \<open>Sequential C-program alphabet\<close>
 
 text 
-{* In order to capture exceptions, we extend the alphabet of UTP by an additional global 
+\<open>In order to capture exceptions, we extend the alphabet of UTP by an additional global 
    state variables:
    \begin{itemize}   
       \<^item> abrupt: a boolean variable used to specify if the program is in an abrupt state or not.
-   \end{itemize}
-*}
+   \end{itemize}\<close>
 
 alphabet abr_vars = 
   abrupt :: bool
 
 declare  abr_vars.splits [alpha_splits]
   
-subsubsection {*Alphabet proofs*}
-text {*
+subsubsection \<open>Alphabet proofs\<close>
+text \<open>
   The two locale interpretations below are a technicality to improve automatic
   proof support via the predicate and relational tactics. This is to enable the
   (re-)interpretation of state spaces to remove any occurrences of lens types
   after the proof tactics @{method pred_simp} and @{method rel_simp}, or any
   of their derivatives have been applied. Eventually, it would be desirable to
   automate both interpretations as part of a custom outer command for defining
-  alphabets.
-*}
+  alphabets.\<close>
 
 interpretation cp_abr:
   lens_interp "\<lambda> (ok, r) . (ok, abrupt\<^sub>v r, more r)"
@@ -62,11 +60,28 @@ apply (rule injI)
 apply (clarsimp)
 done
 
-subsubsection {*Type lifting*}
+subsubsection \<open>Type lifting\<close>
 
-type_synonym '\<alpha> hrel_abr_des  = "'\<alpha> abr_vars_scheme prog"
+type_synonym '\<alpha> abr_prog  = "'\<alpha> abr_vars_scheme prog"
+type_synonym '\<alpha> abr  = "'\<alpha> abr_vars_scheme"
 
-subsubsection {*Syntactic type setup*}
+translations
+  (type) "'\<alpha> abr" <= (type) "'\<alpha> abr_vars_scheme"
+  (type) "'\<alpha> abr" <= (type) "'\<alpha> abr_vars_ext"
+  (type) "'\<alpha> abr_prog" <= (type) "'\<alpha> abr_vars_scheme prog"
+  (type) "'\<alpha> abr_prog" <= (type) "'\<alpha> abr_vars_ext prog"
+
+(*type_synonym '\<alpha> des  = "'\<alpha> des_vars_scheme"
+type_synonym ('\<alpha>, '\<beta>) rel_des = "('\<alpha> des, '\<beta> des) rel"
+type_synonym '\<alpha> hrel_des = "('\<alpha> des) hrel"
+
+translations
+  (type) "'\<alpha> des" <= (type) "'\<alpha> des_vars_scheme"
+  (type) "'\<alpha> des" <= (type) "'\<alpha> des_vars_ext"
+  (type) "('\<alpha>, '\<beta>) rel_des" <= (type) "('\<alpha> des, '\<beta> des) rel"
+  (type) "'\<alpha> hrel_des" <= (type) "'\<alpha> des hrel"*)
+  
+subsubsection \<open>Syntactic type setup\<close>
 
 notation abr_vars_child_lens ("\<Sigma>\<^sub>A\<^sub>B\<^sub>R")
 
@@ -75,24 +90,24 @@ syntax
 translations
   "_svid_st_alpha" => "CONST abr_vars_child_lens"
 
-subsection {*Substitution lift and drop*}
-
+subsection \<open>Substitution lift and drop\<close>
+  
 abbreviation lift_rel_usubst_cpa ("\<lceil>_\<rceil>\<^sub>S\<^sub>A\<^sub>B\<^sub>R")
-where "\<lceil>\<sigma>\<rceil>\<^sub>S\<^sub>A\<^sub>B\<^sub>R \<equiv> \<sigma> \<oplus>\<^sub>s (\<Sigma>\<^sub>A\<^sub>B\<^sub>R \<times>\<^sub>L \<Sigma>\<^sub>A\<^sub>B\<^sub>R)"
+where "\<lceil>\<sigma>\<rceil>\<^sub>S\<^sub>A\<^sub>B\<^sub>R \<equiv> \<sigma> \<oplus>\<^sub>s \<Sigma>\<^sub>A\<^sub>B\<^sub>R "
 
 abbreviation lift_usubst_cpa ("\<lceil>_\<rceil>\<^sub>s\<^sub>A\<^sub>B\<^sub>R")
-where "\<lceil>\<sigma>\<rceil>\<^sub>s\<^sub>A\<^sub>B\<^sub>R \<equiv> \<lceil>\<lceil>\<sigma>\<rceil>\<^sub>s\<rceil>\<^sub>S\<^sub>A\<^sub>B\<^sub>R"
-
+  where "\<lceil>\<sigma>\<rceil>\<^sub>s\<^sub>A\<^sub>B\<^sub>R \<equiv> \<lceil>\<lceil>\<sigma>\<rceil>\<^sub>s\<rceil>\<^sub>S\<^sub>A\<^sub>B\<^sub>R"
+    
 abbreviation drop_cpa_rel_usubst ("\<lfloor>_\<rfloor>\<^sub>S\<^sub>A\<^sub>B\<^sub>R")
-where "\<lfloor>\<sigma>\<rfloor>\<^sub>S\<^sub>A\<^sub>B\<^sub>R \<equiv> \<sigma> \<restriction>\<^sub>s (\<Sigma>\<^sub>A\<^sub>B\<^sub>R \<times>\<^sub>L \<Sigma>\<^sub>A\<^sub>B\<^sub>R)"
+where "\<lfloor>\<sigma>\<rfloor>\<^sub>S\<^sub>A\<^sub>B\<^sub>R \<equiv> \<sigma> \<restriction>\<^sub>s \<Sigma>\<^sub>A\<^sub>B\<^sub>R "
 
 abbreviation drop_cpa_usubst ("\<lfloor>_\<rfloor>\<^sub>s\<^sub>A\<^sub>B\<^sub>R")
 where "\<lfloor>\<sigma>\<rfloor>\<^sub>s\<^sub>A\<^sub>B\<^sub>R \<equiv> \<lfloor>\<lfloor>\<sigma>\<rfloor>\<^sub>S\<^sub>A\<^sub>B\<^sub>R\<rfloor>\<^sub>s"
 
-subsection {*UTP-Relations lift and drop*}
+subsection \<open>UTP-Relations lift and drop\<close>
 
 abbreviation lift_rel_uexpr_cpa ("\<lceil>_\<rceil>\<^sub>A\<^sub>B\<^sub>R")
-where "\<lceil>P\<rceil>\<^sub>A\<^sub>B\<^sub>R \<equiv> P \<oplus>\<^sub>p (\<Sigma>\<^sub>A\<^sub>B\<^sub>R \<times>\<^sub>L \<Sigma>\<^sub>A\<^sub>B\<^sub>R)"
+where "\<lceil>P\<rceil>\<^sub>A\<^sub>B\<^sub>R \<equiv> P \<oplus>\<^sub>p \<Sigma>\<^sub>A\<^sub>B\<^sub>R "
 
 abbreviation lift_pre_uexpr_cpa ("\<lceil>_\<rceil>\<^sub>A\<^sub>B\<^sub>R\<^sub><")
 where "\<lceil>p\<rceil>\<^sub>A\<^sub>B\<^sub>R\<^sub>< \<equiv> \<lceil>\<lceil>p\<rceil>\<^sub><\<rceil>\<^sub>A\<^sub>B\<^sub>R"
@@ -101,7 +116,7 @@ abbreviation lift_post_uexpr_cpa ("\<lceil>_\<rceil>\<^sub>A\<^sub>B\<^sub>R\<^s
 where "\<lceil>p\<rceil>\<^sub>A\<^sub>B\<^sub>R\<^sub>> \<equiv> \<lceil>\<lceil>p\<rceil>\<^sub>>\<rceil>\<^sub>A\<^sub>B\<^sub>R"
 
 abbreviation drop_cpa_rel_uexpr ("\<lfloor>_\<rfloor>\<^sub>A\<^sub>B\<^sub>R")
-where "\<lfloor>P\<rfloor>\<^sub>A\<^sub>B\<^sub>R \<equiv> P \<restriction>\<^sub>p (\<Sigma>\<^sub>A\<^sub>B\<^sub>R \<times>\<^sub>L \<Sigma>\<^sub>A\<^sub>B\<^sub>R)"
+where "\<lfloor>P\<rfloor>\<^sub>A\<^sub>B\<^sub>R \<equiv> P \<restriction>\<^sub>p \<Sigma>\<^sub>A\<^sub>B\<^sub>R"
 
 abbreviation drop_cpa_pre_uexpr ("\<lfloor>_\<rfloor>\<^sub><\<^sub>A\<^sub>B\<^sub>R")
 where "\<lfloor>P\<rfloor>\<^sub><\<^sub>A\<^sub>B\<^sub>R \<equiv> \<lfloor>\<lfloor>P\<rfloor>\<^sub>A\<^sub>B\<^sub>R\<rfloor>\<^sub><"
@@ -109,81 +124,128 @@ where "\<lfloor>P\<rfloor>\<^sub><\<^sub>A\<^sub>B\<^sub>R \<equiv> \<lfloor>\<l
 abbreviation drop_cpa_post_uexpr ("\<lfloor>_\<rfloor>\<^sub>>\<^sub>A\<^sub>B\<^sub>R")
 where "\<lfloor>P\<rfloor>\<^sub>>\<^sub>A\<^sub>B\<^sub>R \<equiv> \<lfloor>\<lfloor>P\<rfloor>\<^sub>A\<^sub>B\<^sub>R\<rfloor>\<^sub>>"
 
-subsection {* Reactive lemmas *}
 
-
-subsection{*Healthiness conditions*}
+subsection \<open>Healthiness conditions\<close>
   
 definition abrh_def [upred_defs]: 
   "abrh(P) = (IF &abrupt THEN SKIP ELSE  P FI)"
 
-section{*Control flow statements*}
+section \<open>Control flow statements\<close>
+  
+subsection \<open>SKIP\<close>
+  
+text \<open>For the below reason we do not re-define skip\<close>
+  
+lemma abrh_skipe[simp]:
+  "abrh(SKIP) = SKIP"
+  unfolding abrh_def
+  by (simp add: if_prog_idem)
 
-subsection{*SKIP*}
+subsection \<open>Assign\<close>
+  
 definition  
-skip_abr_def [urel_defs]: "skip_abr=  abrh(SKIP)"
+assigns_abr_def [urel_defs]: "assigns_abr \<sigma> =  abrh(\<langle>\<sigma>  \<oplus>\<^sub>s \<Sigma>\<^sub>A\<^sub>B\<^sub>R\<rangle>\<^sub>p)"
 
-subsection{*Assign*}
+adhoc_overloading
+  uassigns assigns_abr
 
-definition  
-assigns_abr_def [urel_defs]: "assigns_abr \<sigma> =  abrh(\<langle>\<sigma>\<rangle>\<^sub>p)"
+translations
+  "_assignment xs vs" => "CONST assigns_abr (_mk_usubst (CONST id) xs vs)"
+  "x :== v" <= "CONST assigns_abr (CONST subst_upd (CONST id) (CONST svar x) v)"
 
-subsection{*Throw*}
+subsection \<open>Throw\<close>
 
-definition  
-throw_abr_def [urel_defs]: "throw_abr  =  assigns_abr [&abrupt \<mapsto>\<^sub>s true]"
+definition  throw_abr:: "'a abr_prog" ("THROW")
+where [urel_defs]: "throw_abr  =  passigns (subst_upd id abrupt true)"
 
-subsection{*Sequential composition*}
-text {*It does not need a definition. We get it by type inference.*}  
-term "(throw_abr) ; (p )"  
-subsection{*Conditional composition*}
+subsection \<open>Sequential composition\<close>
+  
+text  \<open>It does not need a definition. We get it by type inference.\<close>  
+  
+subsection \<open>Conditional composition\<close>
+  
+no_notation pcond_prog ("IF (_)/ THEN (_) ELSE (_) FI") 
+  
+definition if_abr :: "'a upred \<Rightarrow> 'a abr_prog \<Rightarrow> 'a abr_prog \<Rightarrow> 'a abr_prog" ("IF (_)/ THEN (_) ELSE (_) FI")
+where [urel_defs]: "if_abr b P Q = pcond_prog (b \<oplus>\<^sub>p \<Sigma>\<^sub>A\<^sub>B\<^sub>R) P Q"
 
-definition  
-if_abr_def [urel_defs]: "if_abr b P Q  =  IF (b \<oplus>\<^sub>p \<Sigma>\<^sub>A\<^sub>B\<^sub>R) THEN P ELSE Q FI"
+subsection \<open>Recursion\<close>
 
-subsection{*Iterations*}
+definition mu_abr:: "('a abr_prog \<Rightarrow> 'a abr_prog) \<Rightarrow> 'a abr_prog"
+where [urel_defs]: "mu_abr P = (\<mu>\<^sub>p X \<bullet> P (abrh X))"
+  
+syntax
+  "_amu" :: "pttrn \<Rightarrow> logic \<Rightarrow> logic" ("\<mu>\<^sub>a _ \<bullet> _" [0, 10] 10)
 
+notation mu_abr ("\<mu>\<^sub>a")
+
+translations
+  "\<mu>\<^sub>a X \<bullet> P" == "CONST mu_abr (\<lambda> X. P)"
+term "mu_abr F"
+term "\<forall>x. abrh x = x"  
+thm normal_design_theory_continuous.LFP_healthy_comp  
+lemma abrh_idem[simp]:"(abrh (abrh X)) = (abrh X)"  
+  unfolding abrh_def
+  by (simp add: if_prog_L6)
+
+lemma lfp_abr_healthy_comp:
+  "\<mu>\<^sub>a F = \<mu>\<^sub>a (F \<circ> abrh)" 
+  unfolding mu_abr_def
+  by simp
+lemma "(abrh (\<mu>\<^sub>a fun1) = (\<mu>\<^sub>a fun1))"
+  unfolding mu_abr_def abrh_def
+     apply (simp only: prog_rep_eq)
+  oops 
+  term "\<Sqinter>\<^bsub>L\<^esub> {u \<in> carrier L. f u \<sqsubseteq>\<^bsub>L\<^esub> u}"    
+ (*I need to re-define LFP such that LFP F = \<Sqinter> {u \<in> {P. abrh P = P}. F u \<sqsubseteq> u}
+   To have such a definition I need to lift \<Sqinter> to prog*)   
+lemma "mono_prog F \<Longrightarrow> F \<in> {P. abrh P = P} \<rightarrow> {P. abrh P = P} \<Longrightarrow> LFP_def = (\<mu>\<^sub>p X \<bullet> P (abrh X))"
+  oops
+lemma "\<And>fun1 fun2. (\<And>x. abrh x = x \<Longrightarrow> (abrh (fun1 x) = (fun1 x)) \<and> fun1 x = fun2 x) \<Longrightarrow> (abrh (\<mu>\<^sub>a fun1) = (\<mu>\<^sub>a fun1)) \<and> \<mu>\<^sub>a fun1 = \<mu>\<^sub>a fun2"
+ oops 
+lemma "mono_prog F \<Longrightarrow> \<mu>\<^sub>a F = F(\<mu>\<^sub>a F)" 
+  apply  mu_abr_def 
+  apply (subst lfp_prog_unfold)
+    
+    thm lfp_prog_unfold[THEN ext]
+       
+subsection \<open>Iterations\<close>
+  
 definition  
 while_abr_def [urel_defs]: "while_abr b I C  = INVR I  WHILE (b \<oplus>\<^sub>p \<Sigma>\<^sub>A\<^sub>B\<^sub>R) \<and> \<not>&abrupt DO C OD"
-
-subsection{*Recursion*}
-(*TODO @Yakoub*)
-
-definition mu_abr_def [urel_defs]:
-  "mu_abr P = (\<mu>\<^sub>p X \<bullet> P (abrh X))"
   
 subsection {*Try catch*}
-
+term "passigns (subst_upd id abrupt (\<not> &abrupt))"
 definition  try_catch_abr_def [urel_defs]:
   "try_catch_abr P Q = 
-   abrh (P ;  IF &abrupt THEN (abrupt:== (\<not> &abrupt) ; abrh(Q)) ELSE skip_abr FI)"
+   abrh (P ;  IF &abrupt THEN (passigns (subst_upd id abrupt (\<not> &abrupt)) ; abrh(Q)) ELSE SKIP FI)"
 
 section {*algebraic laws*} 
 
 lemma [algebraic_laws_prog]:"IF b THEN P ELSE P FI = P"
   by (simp add: prog_rep_eq Algebraic_Laws.cond_idem)
 
-lemma [algebraic_laws_prog]:"skip_abr ;  P =  P" "P ; skip_abr = P"
-  unfolding skip_abr_def abrh_def
-  by (simp add: algebraic_laws_prog)+  
+lemma [algebraic_laws_prog]:"SKIP ;  P =  P" "P ; SKIP = P"
+  unfolding  abrh_def
+  by (simp_all)  
 
 lemma [algebraic_laws_prog]:"throw_abr ;  (abrh P) = throw_abr"     
-  unfolding throw_abr_def abrh_def assigns_abr_def skip_abr_def
+  unfolding throw_abr_def abrh_def assigns_abr_def 
   apply (simp add: prog_rep_eq) 
    apply rel_auto
   done
 
-lemma "abrh(\<langle>a\<rangle>\<^sub>p) ; abrh (throw_abr ;  IF &abrupt THEN (abrupt:== (\<not> &abrupt) ; abrh(\<langle>b\<rangle>\<^sub>p)) ELSE skip_abr FI) = 
+lemma "abrh(\<langle>a\<rangle>\<^sub>p) ; abrh (throw_abr ;  IF &abrupt THEN (passigns (subst_upd id abrupt (\<not> &abrupt)) ; abrh(\<langle>b\<rangle>\<^sub>p)) ELSE SKIP FI) = 
          (abrh(\<langle>a\<rangle>\<^sub>p); abrh(\<langle>b\<rangle>\<^sub>p))"
-  unfolding throw_abr_def abrh_def assigns_abr_def skip_abr_def
+  unfolding throw_abr_def abrh_def assigns_abr_def 
     apply (simp add: prog_rep_eq) 
   apply rel_auto
   apply (smt abr_vars.ext_inject abr_vars_ext_def)+
   done  
  
-lemma "abrh(P) ; abrh (throw_abr ;  IF &abrupt THEN (abrupt:== (\<not> &abrupt) ; abrh(Q)) ELSE skip_abr FI) = 
+lemma "abrh(P) ; abrh (throw_abr ;  IF &abrupt THEN (passigns (subst_upd id abrupt (\<not> &abrupt)) ; abrh(Q)) ELSE SKIP FI) = 
          (abrh(P); abrh(Q))"
-  unfolding throw_abr_def abrh_def assigns_abr_def skip_abr_def
+  unfolding throw_abr_def abrh_def assigns_abr_def 
     apply (simp add: prog_rep_eq) 
   apply rel_auto
   apply transfer
